compactness: more

Splitting_Framework/Harrison_FOL_Compactness.thy
@@ -12,7 +12,7 @@ begin
 (* This heavily reuses Ghilain's FOL_Compactness code, with simplifications for nat type
    and renamings to follow Harrison's text *)
 
-(* Comments starting with != indicate discrepencies with Harrison's formalisation *)
+(* Comments starting with != indicate discrepancies with Harrison's formalisation *)
 
 
 type_synonym nterm = \<open>(nat, nat) term\<close>
@@ -81,9 +81,12 @@ abbreviation FVT :: \<open>nterm \<Rightarrow> nat set\<close> where
 
 fun FV :: \<open>form \<Rightarrow> nat set\<close> where
   \<open>FV \<^bold>\<bottom> = {}\<close>
-| \<open>FV (Atom _ args') = (\<Union> a \<in> set args'. FVT a)\<close>
+| \<open>FV (Atom _ ts) = (\<Union> a \<in> set ts. FVT a)\<close>
 | \<open>FV (\<phi> \<^bold>\<longrightarrow> \<psi>) = FV \<phi> \<union> FV \<psi>\<close>
 | \<open>FV (\<^bold>\<forall> x\<^bold>. \<phi>) = FV \<phi> - {x}\<close>
+
+lemma FV_all_subs: \<open>FV \<phi> \<subseteq> FV (\<^bold>\<forall> x\<^bold>. \<phi>) \<union> {x}\<close>
+  by fastforce
 
 lemma finite_FV: \<open>finite (FV \<phi>)\<close>
   by (induction \<phi>, auto)
@@ -109,8 +112,37 @@ fun formsubst :: \<open>form \<Rightarrow> (nat, nat) subst \<Rightarrow> form\<
 | \<open>(\<^bold>\<forall> x\<^bold>. \<phi>) \<cdot>\<^sub>f\<^sub>m \<sigma> =
     (let \<sigma>' = \<sigma>(x := Var x);
          z = if \<exists> y. y \<in> FV (\<^bold>\<forall> x\<^bold>. \<phi>) \<and> x \<in> FVT (\<sigma>' y)
-             then variant (FV (\<^bold>\<forall> x\<^bold>. \<phi>)) else x in
+             then variant (FV (\<phi> \<cdot>\<^sub>f\<^sub>m \<sigma>')) else x in
     \<^bold>\<forall> z\<^bold>. (\<phi> \<cdot>\<^sub>f\<^sub>m \<sigma>(x := Var z)))\<close>
+
+fun formsubst2 :: \<open>form \<Rightarrow> (nat, nat) subst \<Rightarrow> form\<close> (infixl \<open>\<cdot>\<^sub>f\<^sub>m2\<close> 75) where
+  \<open>\<^bold>\<bottom> \<cdot>\<^sub>f\<^sub>m2 _ = \<^bold>\<bottom>\<close> 
+| \<open>(Atom p ts) \<cdot>\<^sub>f\<^sub>m2 \<sigma> = Atom p [t \<cdot> \<sigma>. t \<leftarrow> ts]\<close>
+| \<open>(\<phi> \<^bold>\<longrightarrow> \<psi>) \<cdot>\<^sub>f\<^sub>m2 \<sigma> = (\<phi> \<cdot>\<^sub>f\<^sub>m2 \<sigma>) \<^bold>\<longrightarrow> (\<psi> \<cdot>\<^sub>f\<^sub>m2 \<sigma>)\<close>
+| \<open>(\<^bold>\<forall> x\<^bold>. \<phi>) \<cdot>\<^sub>f\<^sub>m2 \<sigma> = (let \<sigma>' = \<sigma>(x := Var x) in
+    (if \<exists> y. y \<in> FV (\<^bold>\<forall> x\<^bold>. \<phi>) \<and> x \<in> FVT (\<sigma>' y)
+    then (let z = variant (FV (\<phi> \<cdot>\<^sub>f\<^sub>m2 \<sigma>')) in
+      \<^bold>\<forall> z\<^bold>. (\<phi> \<cdot>\<^sub>f\<^sub>m2 \<sigma>(x := Var z)))
+    else \<^bold>\<forall> x\<^bold>. (\<phi> \<cdot>\<^sub>f\<^sub>m2 \<sigma>')))\<close>
+
+lemma formsubst_def_switch: \<open>\<phi> \<cdot>\<^sub>f\<^sub>m \<sigma> = \<phi> \<cdot>\<^sub>f\<^sub>m2 \<sigma>\<close>
+proof (induction \<phi> arbitrary: \<sigma> rule: form.induct)
+  case Bot
+  then show ?case
+    by fastforce
+next
+  case (Atom x1 x2)
+  then show ?case
+    by fastforce
+next
+  case (Implies x1 x2)
+  then show ?case
+    by fastforce
+next
+  case (Forall x1 x2)
+  then show ?case
+    by (smt (verit, best) formsubst.simps(4) formsubst2.simps(4))
+qed
 
 lemma termsubst_valuation: \<open>\<forall>x\<in>FVT t. \<sigma> x = \<sigma>' x \<Longrightarrow> t \<cdot> \<sigma> = t \<cdot> \<sigma>'\<close>
   using eval_same_vars by blast
@@ -142,10 +174,10 @@ next
   show ?case
   proof (cases \<open>\<exists> y. y \<in> FV (\<^bold>\<forall> x\<^bold>. \<phi>) \<and> x \<in> FVT (\<sigma>'' y)\<close>)
     case True
-    then have \<open>(\<^bold>\<forall> x\<^bold>. \<phi>) \<cdot>\<^sub>f\<^sub>m \<sigma> = (let z = variant (FV (\<^bold>\<forall> x\<^bold>. \<phi>)) in \<^bold>\<forall> z\<^bold>. (\<phi> \<cdot>\<^sub>f\<^sub>m \<sigma>(x := Var z)))\<close>
+    then have \<open>(\<^bold>\<forall> x\<^bold>. \<phi>) \<cdot>\<^sub>f\<^sub>m \<sigma> = (let z = variant (FV (\<phi> \<cdot>\<^sub>f\<^sub>m \<sigma>'')) in \<^bold>\<forall> z\<^bold>. (\<phi> \<cdot>\<^sub>f\<^sub>m \<sigma>(x := Var z)))\<close>
       by (simp add: \<sigma>''_def)
-    also have \<open>... = (let z = variant (FV (\<^bold>\<forall> x\<^bold>. \<phi>)) in \<^bold>\<forall> z\<^bold>. (\<phi> \<cdot>\<^sub>f\<^sub>m \<sigma>'(x := Var z)))\<close>
-      using sig_x_subst by (metis Forall.IH)
+    also have \<open>... = (let z = variant (FV (\<phi> \<cdot>\<^sub>f\<^sub>m \<sigma>''')) in \<^bold>\<forall> z\<^bold>. (\<phi> \<cdot>\<^sub>f\<^sub>m \<sigma>'(x := Var z)))\<close>
+      using sig_x_subst \<sigma>'''_def by (metis Forall.IH \<sigma>''_def)
     also have \<open>... = (\<^bold>\<forall> x\<^bold>. \<phi>) \<cdot>\<^sub>f\<^sub>m \<sigma>'\<close>
       using True \<sigma>'''_def ex_var_equiv formsubst.simps(4) by presburger
     finally show ?thesis .
@@ -160,12 +192,8 @@ qed
 lemma \<open>{x. \<exists>y. y \<in> (s \<union> t) \<and> P x y} = {x. \<exists>y. y \<in> s \<and> P x y} \<union> {x. \<exists>y. y \<in> t \<and> P x y}\<close>
   by blast
 
-
 lemma \<open>FV (\<phi> \<cdot>\<^sub>f\<^sub>m \<sigma>) = {x. \<exists>y. y \<in> (FV \<phi>) \<and> x \<in> FVT ((Var y) \<cdot> \<sigma>)}\<close>
 proof (induction \<phi> arbitrary: \<sigma> rule:form.induct)
-  case Bot
-  then show ?case by simp
-next
   case (Atom x1 x2)
   have \<open>FV (Atom x1 x2 \<cdot>\<^sub>f\<^sub>m \<sigma>) = (\<Union>a \<in> set x2. FVT (a  \<cdot> \<sigma>))\<close>
     by auto
@@ -197,55 +225,375 @@ next
     by auto
   finally show ?case .
 next
-  case (Implies \<phi>1 \<phi>2)
-  then show ?case by auto
+  case (Forall x \<phi>)
+  define \<sigma>' where "\<sigma>' = \<sigma>(x := Var x)"
+  show ?case
+  proof (cases "\<exists> y. y \<in> FV (\<^bold>\<forall> x\<^bold>. \<phi>) \<and> x \<in> FVT (\<sigma>' y)")
+    case True
+    then obtain y where y_in: \<open>y \<in> FV (\<^bold>\<forall> x\<^bold>. \<phi>)\<close> and x_in: \<open>x \<in> FVT (\<sigma>' y)\<close>
+      by blast
+    then have y_neq_x: \<open>y \<noteq> x\<close> by simp
+    then have y_in2: \<open>y \<in> FV \<phi>\<close>
+      using y_in by fastforce
+    have x_in2: \<open>x \<in> FVT (Var y \<cdot> \<sigma>)\<close>
+      using x_in y_neq_x unfolding \<sigma>'_def by simp
+  
+    define z where "z = variant (FV (\<phi> \<cdot>\<^sub>f\<^sub>m \<sigma>'))"
+    have x_in3: \<open>x \<in> FVT (Var y \<cdot> \<sigma>(x := Var z))\<close>
+      using x_in2 y_neq_x by simp
+
+    have \<open>(\<^bold>\<forall> x\<^bold>. \<phi>) \<cdot>\<^sub>f\<^sub>m \<sigma> = \<^bold>\<forall> z\<^bold>. (\<phi> \<cdot>\<^sub>f\<^sub>m \<sigma>(x := Var z))\<close>
+      using z_def formsubst_def_switch
+      by (smt (verit, ccfv_threshold) True \<sigma>'_def formsubst.simps(4))
+    then have \<open>FV ((\<^bold>\<forall> x\<^bold>. \<phi>) \<cdot>\<^sub>f\<^sub>m \<sigma>) = {xa. \<exists>y. y \<in> FV \<phi> \<and> xa \<in> FVT (Var y \<cdot> \<sigma>(x := Var z))} - {z}\<close>
+      using Forall[of "\<sigma>(x := Var z)"] using FV.simps(4) by presburger
+    also have \<open>... = {xa. \<exists>y. y \<in> FV \<phi> - {x} \<and> xa \<in> FVT (Var y \<cdot> \<sigma>)}\<close>
+    proof
+      show \<open>{xa. \<exists>y. y \<in> FV \<phi> \<and> xa \<in> FVT (Var y \<cdot> \<sigma>(x := Var z))} - {z} \<subseteq> 
+        {xa. \<exists>y. y \<in> FV \<phi> - {x} \<and> xa \<in> FVT (Var y \<cdot> \<sigma>)}\<close>
+      proof
+        fix xa
+        assume xa_in: \<open>xa \<in> {xa. \<exists>y. y \<in> FV \<phi> \<and> xa \<in> FVT (Var y \<cdot> \<sigma>(x := Var z))} - {z}\<close>
+        then obtain ya where ya_in: \<open>ya \<in> FV \<phi>\<close> and xa_image: \<open>xa \<in> FVT (Var ya \<cdot> \<sigma>(x := Var z))\<close>
+          by blast
+        have ya_neq_x: \<open>ya \<noteq> x\<close> using xa_image xa_in by fastforce
+        then have \<open>xa \<in> FVT (Var ya \<cdot> \<sigma>)\<close> using xa_image by simp
+        moreover have \<open>ya \<in> FV \<phi> - {x}\<close>
+          using ya_neq_x ya_in by blast
+        ultimately show \<open>xa \<in> {xa. \<exists>y. y \<in> FV \<phi> - {x} \<and> xa \<in> FVT (Var y \<cdot> \<sigma>)}\<close>
+          by auto
+      qed
+    next
+      show \<open>{xa. \<exists>y. y \<in> FV \<phi> - {x} \<and> xa \<in> FVT (Var y \<cdot> \<sigma>)} \<subseteq> 
+        {xa. \<exists>y. y \<in> FV \<phi> \<and> xa \<in> FVT (Var y \<cdot> \<sigma>(x := Var z))} - {z}\<close>
+      proof
+        fix xa
+        assume xa_in: \<open>xa \<in> {xa. \<exists>y. y \<in> FV \<phi> - {x} \<and> xa \<in> FVT (Var y \<cdot> \<sigma>)}\<close>
+        then obtain ya where ya_in:  \<open>ya \<in> FV \<phi> - {x}\<close> and xa_image: \<open>xa \<in> FVT (Var ya \<cdot> \<sigma>)\<close>
+          by blast
+        have ya_neq: \<open>ya \<noteq> x\<close> using ya_in by blast
+        then have xa_in2: \<open>xa \<in> FVT (Var ya \<cdot> \<sigma>(x := Var z))\<close> using xa_image by simp
+        then have \<open>xa \<in> FV (\<phi> \<cdot>\<^sub>f\<^sub>m \<sigma>(x := Var z))\<close> 
+          using ya_in Forall by force
+        then have \<open>xa \<in> FV (\<phi> \<cdot>\<^sub>f\<^sub>m \<sigma>')\<close>
+          using ya_neq Forall xa_image ya_in unfolding \<sigma>'_def by auto
+        then have \<open>xa \<noteq> z\<close> using z_def unfolding variant_def
+          by (metis Max_ge Suc_eq_plus1 finite_FV lessI less_le_not_le)
+        moreover have \<open>ya \<in> FV \<phi>\<close> using ya_in by blast
+        ultimately show \<open>xa \<in> {xa. \<exists>y. y \<in> FV \<phi> \<and> xa \<in> FVT (Var y \<cdot> \<sigma>(x := Var z))} - {z}\<close>
+          using xa_in2 by blast
+      qed
+    qed
+    finally show ?thesis by simp
+  next
+    case False
+    then have \<open>(\<^bold>\<forall> x\<^bold>. \<phi>) \<cdot>\<^sub>f\<^sub>m \<sigma> = \<^bold>\<forall> x\<^bold>. (\<phi> \<cdot>\<^sub>f\<^sub>m \<sigma>')\<close>
+      using formsubst_def_switch \<sigma>'_def by fastforce
+    then have \<open>FV ((\<^bold>\<forall> x\<^bold>. \<phi>) \<cdot>\<^sub>f\<^sub>m \<sigma>) = {z. \<exists>y. y \<in> FV \<phi> \<and> z \<in> FVT (Var y \<cdot> \<sigma>')} - {x}\<close>
+      using Forall by simp
+    also have \<open>... = {z. \<exists>y. y \<in> FV (\<^bold>\<forall> x\<^bold>. \<phi>) \<and> z \<in> FVT (Var y \<cdot> \<sigma>)}\<close>
+      using False unfolding \<sigma>'_def by auto
+    finally show ?thesis .
+  qed
+qed auto
+
+
+locale struct =
+  fixes
+    M :: \<open>'m set\<close> and
+    FN :: \<open>nat \<Rightarrow> 'm list \<Rightarrow> 'm\<close> and
+    REL :: \<open>nat \<Rightarrow> 'm list set\<close> 
+  assumes
+    M_nonempty: \<open>M \<noteq> {}\<close> and 
+    FN_dom_to_dom: \<open>\<forall> f es. (\<forall> e \<in> set es. e \<in> M) \<longrightarrow> FN f es \<in> M\<close> and
+    REL_to_dom: \<open>\<forall> p. \<forall> es \<in> REL p. \<forall> e \<in> set es. e \<in> M\<close> 
+
+definition is_vars :: \<open>'m set \<Rightarrow> (nat \<Rightarrow> 'm) \<Rightarrow> bool\<close> where
+  [simp]: \<open>is_vars M \<beta> \<longleftrightarrow> (\<forall> v. \<beta> v \<in> M)\<close> 
+
+typedef 'm intrp =
+  \<open>{ (M :: 'm set, FN :: nat \<Rightarrow> 'm list \<Rightarrow> 'm, REL :: nat \<Rightarrow> 'm list set). struct M FN REL }\<close>
+  using struct.intro
+  by fastforce
+
+setup_lifting type_definition_intrp
+
+lift_definition dom :: \<open>'m intrp \<Rightarrow> 'm set\<close> is fst .
+lift_definition interp_fn :: \<open>'m intrp \<Rightarrow> (nat \<Rightarrow> 'm list \<Rightarrow> 'm)\<close> is \<open>fst \<circ> snd\<close> .
+lift_definition interp_rel :: \<open>'m intrp \<Rightarrow> (nat \<Rightarrow> 'm list set)\<close> is \<open>snd \<circ> snd\<close> .
+
+lemma intrp_is_struct: \<open>struct (dom \<M>) (interp_fn \<M>) (interp_rel \<M>)\<close>
+  by transfer auto 
+
+lemma dom_Abs_is_fst [simp]: \<open>struct M FN REL \<Longrightarrow> dom (Abs_intrp (M, FN, REL)) = M\<close>
+  by (simp add: Abs_intrp_inverse dom.rep_eq) 
+
+lemma interp_fn_Abs_is_fst_snd [simp]: \<open>struct M FN REL \<Longrightarrow> interp_fn (Abs_intrp (M, FN, REL)) = FN\<close>
+  by (simp add: Abs_intrp_inverse interp_fn.rep_eq) 
+
+lemma interp_rel_Abs_is_snd_snd [simp]: 
+  \<open>struct M FN REL \<Longrightarrow> interp_rel (Abs_intrp (M, FN, REL)) = REL\<close>
+  by (simp add: Abs_intrp_inverse interp_rel.rep_eq) 
+
+lemma FN_dom_to_dom: \<open>\<forall> t \<in> set ts. t \<in> dom \<M> \<Longrightarrow> interp_fn \<M> f ts \<in> dom \<M>\<close>
+  by (meson intrp_is_struct struct.FN_dom_to_dom) 
+
+fun eval
+  :: \<open>nterm \<Rightarrow> 'm intrp \<Rightarrow> (nat \<Rightarrow> 'm) \<Rightarrow> 'm\<close>
+  (\<open>\<lbrakk>_\<rbrakk>\<^bsup>_,_\<^esup>\<close> [50, 0, 0] 70) where
+  \<open>\<lbrakk>Var v\<rbrakk>\<^bsup>_,\<beta>\<^esup> = \<beta> v\<close>
+| \<open>\<lbrakk>Fun f ts\<rbrakk>\<^bsup>\<M>,\<beta>\<^esup> = interp_fn \<M> f [\<lbrakk>t\<rbrakk>\<^bsup>\<M>,\<beta>\<^esup>. t \<leftarrow> ts]\<close> 
+
+fun holds
+  :: \<open>'m intrp \<Rightarrow> (nat \<Rightarrow> 'm) \<Rightarrow> form \<Rightarrow> bool\<close> (\<open>_,_ \<Turnstile> _\<close> [30, 30, 80] 80) where
+  \<open>\<M>,\<beta> \<Turnstile> \<^bold>\<bottom> \<longleftrightarrow> False\<close>
+| \<open>\<M>,\<beta> \<Turnstile> Atom p ts \<longleftrightarrow> [\<lbrakk>t\<rbrakk>\<^bsup>\<M>,\<beta>\<^esup>. t \<leftarrow> ts] \<in> interp_rel \<M> p\<close>
+| \<open>\<M>,\<beta> \<Turnstile> \<phi> \<^bold>\<longrightarrow> \<psi> \<longleftrightarrow> ((\<M>,\<beta> \<Turnstile> \<phi>) \<longrightarrow> (\<M>,\<beta> \<Turnstile> \<psi>))\<close>
+| \<open>\<M>,\<beta> \<Turnstile> (\<^bold>\<forall> x\<^bold>. \<phi>) \<longleftrightarrow> (\<forall>a \<in> dom \<M>. \<M>,\<beta>(x := a) \<Turnstile> \<phi>)\<close>
+
+lemma holds_indep_\<beta>_if:
+  \<open>\<forall> v \<in> FV \<phi>. \<beta>\<^sub>1 v = \<beta>\<^sub>2 v \<Longrightarrow> \<M>,\<beta>\<^sub>1 \<Turnstile> \<phi> \<longleftrightarrow> \<M>,\<beta>\<^sub>2 \<Turnstile> \<phi>\<close>
+proof (induction \<phi> arbitrary: \<beta>\<^sub>1 \<beta>\<^sub>2)
+  case Bot
+  then show ?case
+    by simp
+next
+  case (Atom p ts)
+  then have \<open>\<forall> t \<in> set ts. \<forall> v \<in> FVT t. \<beta>\<^sub>1 v = \<beta>\<^sub>2 v\<close>
+    by simp 
+  then have \<open>[\<lbrakk>t\<rbrakk>\<^bsup>\<M>,\<beta>\<^sub>1\<^esup>. t \<leftarrow> ts] = [\<lbrakk>t\<rbrakk>\<^bsup>\<M>,\<beta>\<^sub>2\<^esup>. t \<leftarrow> ts]\<close>
+  proof (induction ts) 
+    case Nil
+    then show ?case
+      by simp
+  next
+    case (Cons a ts)
+    then show ?case
+    proof (induction a)
+      case (Var x)
+      then show ?case
+        by simp 
+    next
+      case (Fun f ts')
+      then have \<open>\<forall> t \<in> set ts'. \<forall> v \<in> FVT t. \<beta>\<^sub>1 v = \<beta>\<^sub>2 v\<close>
+        by simp 
+      then have \<open>[\<lbrakk>t\<rbrakk>\<^bsup>\<M>,\<beta>\<^sub>1\<^esup>. t \<leftarrow> ts'] = [\<lbrakk>t\<rbrakk>\<^bsup>\<M>,\<beta>\<^sub>2\<^esup>. t \<leftarrow> ts']\<close>
+        using Cons.IH Fun.IH Fun.prems(2)
+        by force
+      then have \<open>interp_fn \<M> f [\<lbrakk>t\<rbrakk>\<^bsup>\<M>,\<beta>\<^sub>1\<^esup>. t \<leftarrow> ts'] = interp_fn \<M> f [\<lbrakk>t\<rbrakk>\<^bsup>\<M>,\<beta>\<^sub>2\<^esup>. t \<leftarrow> ts']\<close>
+        by argo 
+      then show ?case
+        using Cons.IH Fun.prems(2)
+        by force 
+    qed
+  qed
+  then have \<open>[\<lbrakk>t\<rbrakk>\<^bsup>\<M>,\<beta>\<^sub>1\<^esup>. t \<leftarrow> ts] \<in> interp_rel \<M> p \<longleftrightarrow> [\<lbrakk>t\<rbrakk>\<^bsup>\<M>,\<beta>\<^sub>2\<^esup>. t \<leftarrow> ts] \<in> interp_rel \<M> p\<close>
+    by argo
+  then show ?case
+    by simp
+next
+  case (Implies \<phi> \<psi>)
+  then have
+    \<open>\<forall>v \<in> FV \<phi>. \<beta>\<^sub>1 v = \<beta>\<^sub>2 v\<close> and
+    \<open>\<forall>v \<in> FV \<psi>. \<beta>\<^sub>1 v = \<beta>\<^sub>2 v\<close>
+    by auto
+  then have
+    \<open>\<M>,\<beta>\<^sub>1 \<Turnstile> \<phi> \<longleftrightarrow> \<M>,\<beta>\<^sub>2 \<Turnstile> \<phi>\<close> and
+    \<open>\<M>,\<beta>\<^sub>1 \<Turnstile> \<psi> \<longleftrightarrow> \<M>,\<beta>\<^sub>2 \<Turnstile> \<psi>\<close>
+    using Implies.IH by auto
+  then show ?case
+    by simp
+next
+  case (Forall x \<phi>)
+  then have \<open>\<forall>a \<in> dom \<M>. (\<M>,\<beta>\<^sub>1(x := a) \<Turnstile> \<phi>) = (\<M>,\<beta>\<^sub>2(x := a) \<Turnstile> \<phi>)\<close>
+    by simp
+  then show ?case 
+    by simp
+qed
+
+lemma holds_indep_intrp_if:
+  fixes
+    \<phi> :: form and
+    \<M> \<M>' :: \<open>'m intrp\<close> 
+  assumes
+    dom_eq: \<open>dom \<M> = dom \<M>'\<close> and
+    rel_eq: \<open>\<forall> p. interp_rel \<M> p = interp_rel \<M>' p\<close> and
+    fn_eq: \<open>\<forall> f ts. (f, length ts) \<in> functions_form \<phi> \<longrightarrow> interp_fn \<M> f ts = interp_fn \<M>' f ts\<close>
+  shows
+    \<open>\<forall>\<beta>.  \<M>,\<beta> \<Turnstile> \<phi> \<longleftrightarrow> \<M>',\<beta> \<Turnstile> \<phi>\<close>
+  using fn_eq
+proof (intro allI impI, induction \<phi>)
+  case (Atom p ts)
+
+  have all_fn_sym_in: \<open>(\<Union> t \<in> set ts. functions_term t) \<subseteq> functions_form (Atom p ts)\<close> (is \<open>?A \<subseteq> _\<close>)
+    by simp 
+
+  have eval_tm_eq: \<open>\<lbrakk>t\<rbrakk>\<^bsup>\<M>,\<beta>\<^esup> = \<lbrakk>t\<rbrakk>\<^bsup>\<M>',\<beta>\<^esup>\<close>
+    if \<open>functions_term t \<subseteq> functions_form (Atom p ts)\<close> 
+    for t 
+    using that
+  proof (induction t) 
+    case (Fun f ts') 
+
+    have \<open>\<forall> t' \<in> set ts'. functions_term t' \<subseteq> functions_form (Atom p ts)\<close>
+      using Fun.prems
+      by auto
+    moreover have \<open>(f, length [\<lbrakk>t'\<rbrakk>\<^bsup>\<M>,\<beta>\<^esup>. t' \<leftarrow> ts']) \<in> functions_form (Atom p ts)\<close>
+      using Fun.prems
+      by fastforce 
+    ultimately show ?case
+      using Fun.IH Atom.prems(1)[rule_format, of f \<open>[\<lbrakk>t'\<rbrakk>\<^bsup>\<M>,\<beta>\<^esup>. t' \<leftarrow> ts']\<close>] 
+      by (smt (verit, del_insts) eval.simps(2) map_eq_conv)
+  qed auto 
+
+  have \<open>\<M>,\<beta> \<Turnstile> Atom p ts \<longleftrightarrow> [\<lbrakk>t\<rbrakk>\<^bsup>\<M>,\<beta>\<^esup>. t \<leftarrow> ts] \<in> interp_rel \<M> p\<close>
+    by simp
+  also have \<open>... \<longleftrightarrow> [\<lbrakk>t\<rbrakk>\<^bsup>\<M>,\<beta>\<^esup>. t \<leftarrow> ts] \<in> interp_rel \<M>' p\<close>
+    by (simp add: rel_eq)
+  also have \<open>... \<longleftrightarrow> [\<lbrakk>t\<rbrakk>\<^bsup>\<M>',\<beta>\<^esup>. t \<leftarrow> ts] \<in> interp_rel \<M>' p\<close>
+    using eval_tm_eq all_fn_sym_in
+    by (metis (mono_tags, lifting) UN_subset_iff map_eq_conv)
+  also have \<open>... \<longleftrightarrow> \<M>',\<beta> \<Turnstile> Atom p ts\<close>
+    by auto 
+  finally show ?case .
+next
+  case (Forall x \<phi>)
+
+  have \<open>\<M>,\<beta> \<Turnstile> (\<^bold>\<forall> x\<^bold>. \<phi>) \<longleftrightarrow> (\<forall> a \<in> dom \<M>. \<M>,\<beta>(x := a) \<Turnstile> \<phi>)\<close>
+    by simp 
+  also have \<open>... = (\<forall> a \<in> dom \<M>. \<M>',\<beta>(x := a) \<Turnstile> \<phi>)\<close>
+    using Forall.IH Forall.prems by simp
+  also have \<open>... = (\<forall> a \<in> dom \<M>'. \<M>',\<beta>(x := a) \<Turnstile> \<phi>)\<close>
+    by (simp add: dom_eq)
+  also have \<open>... = (\<M>',\<beta> \<Turnstile> (\<^bold>\<forall> x\<^bold>. \<phi>))\<close>
+    by auto 
+  finally show ?case . 
+qed auto
+
+abbreviation (input) \<open>eval_subst \<M> \<beta> \<sigma> v \<equiv> \<lbrakk>\<sigma> v\<rbrakk>\<^bsup>\<M>,\<beta>\<^esup>\<close>
+
+lemma subst_lemma_terms: \<open>\<lbrakk>t \<cdot> \<sigma>\<rbrakk>\<^bsup>\<M>,\<beta>\<^esup> = \<lbrakk>t\<rbrakk>\<^bsup>\<M>,eval_subst \<M> \<beta> \<sigma>\<^esup>\<close>
+proof (induction t)
+  case (Var v)
+  then show ?case
+    by auto 
+next
+  case (Fun f ts)
+
+  have \<open>\<lbrakk>Fun f ts \<cdot> \<sigma>\<rbrakk>\<^bsup>\<M>,\<beta>\<^esup> = \<lbrakk>Fun f [t \<cdot> \<sigma>. t \<leftarrow> ts]\<rbrakk>\<^bsup>\<M>,\<beta>\<^esup>\<close>
+    by auto
+  also have \<open>... = interp_fn \<M> f [\<lbrakk>t\<rbrakk>\<^bsup>\<M>,\<beta>\<^esup>. t \<leftarrow> [t \<cdot> \<sigma>. t \<leftarrow> ts]]\<close>
+    by auto 
+  also have \<open>... = interp_fn \<M> f [\<lbrakk>t \<cdot> \<sigma>\<rbrakk>\<^bsup>\<M>,\<beta>\<^esup>. t \<leftarrow> ts]\<close>
+    unfolding map_map
+    by (meson comp_apply)
+  also have \<open>... = interp_fn \<M> f [\<lbrakk>t\<rbrakk>\<^bsup>\<M>,eval_subst \<M> \<beta> \<sigma>\<^esup>. t \<leftarrow> ts]\<close>
+    using Fun.IH
+    by (smt (verit, best) map_eq_conv) 
+  also have \<open>... = \<lbrakk>Fun f ts\<rbrakk>\<^bsup>\<M>,eval_subst \<M> \<beta> \<sigma>\<^esup>\<close>
+    by auto 
+  finally show ?case .
+qed
+
+lemma eval_indep_\<beta>_if:
+  assumes \<open>\<forall> v \<in> FVT t. \<beta> v = \<beta>' v\<close>
+  shows \<open>\<lbrakk>t\<rbrakk>\<^bsup>\<M>,\<beta>\<^esup> = \<lbrakk>t\<rbrakk>\<^bsup>\<M>,\<beta>'\<^esup>\<close>
+    using assms
+proof (induction t)
+  case (Var v)
+  then show ?case
+    by auto 
+next
+  case (Fun f ts)
+  then show ?case
+    by (smt (verit, ccfv_SIG) eval.simps(2) map_eq_conv term.set_intros(4)) 
+qed
+
+lemma concat_map: \<open>[f t. t \<leftarrow> [g t. t \<leftarrow> ts]] = [f (g t). t \<leftarrow> ts]\<close> by simp
+
+find_theorems "_(_ := _)" name: Term
+
+lemma \<open>\<nexists>y. x \<in> FVT (\<sigma> y) \<Longrightarrow> \<sigma> x = Var x \<Longrightarrow> (\<lambda>v. \<lbrakk>\<sigma> v\<rbrakk>\<^bsup>\<M>,\<beta>(x := a)\<^esup>) = (\<lambda>v. \<lbrakk>\<sigma> v\<rbrakk>\<^bsup>\<M>,\<beta>\<^esup>)(x := a)\<close>
+proof
+  fix v
+  assume x_idem: \<open>\<sigma> x = Var x\<close> and
+    case_false: \<open>\<nexists>y. x \<in> FVT (\<sigma> y)\<close>
+  show \<open>\<lbrakk>\<sigma> v\<rbrakk>\<^bsup>\<M>,\<beta>(x := a)\<^esup> = ((\<lambda>v. \<lbrakk>\<sigma> v\<rbrakk>\<^bsup>\<M>,\<beta>\<^esup>)(x := a)) v\<close>
+  proof (induction "\<sigma> v")
+    case (Var y)
+    then show ?case
+      proof (cases "y=x")
+        case True
+        then have \<open>\<lbrakk>\<sigma> v\<rbrakk>\<^bsup>\<M>,\<beta>(x := a)\<^esup> = a\<close>
+          using Var by simp
+        have \<open>((\<lambda>v. \<lbrakk>\<sigma> v\<rbrakk>\<^bsup>\<M>,\<beta>\<^esup>)(x := a)) v = (if v = x then a else \<lbrakk>\<sigma> v\<rbrakk>\<^bsup>\<M>,\<beta>\<^esup>)\<close>
+          by simp
+        have 
+        then have \<open>((\<lambda>v. \<lbrakk>\<sigma> v\<rbrakk>\<^bsup>\<M>,\<beta>\<^esup>)(x := a)) v = a\<close>
+          using True Var x_idem
+          sorry
+        then show ?thesis sorry
+      next
+        case False
+        then show ?thesis sorry
+      qed
+  next
+    case (Fun x1a x2)
+    then show ?case sorry
+  qed
+qed
+
+
+lemma swap_subst_eval: \<open>\<M>,\<beta> \<Turnstile> (\<phi> \<cdot>\<^sub>f\<^sub>m \<sigma>) \<longleftrightarrow> \<M>,(\<lambda>v. eval_subst \<M> \<beta> \<sigma> v) \<Turnstile> \<phi>\<close>
+proof (induction \<phi> arbitrary: \<sigma> \<beta>)
+  case (Atom p ts)
+  have \<open>\<M>,\<beta> \<Turnstile> (Atom p ts \<cdot>\<^sub>f\<^sub>m \<sigma>) \<longleftrightarrow> \<M>,\<beta> \<Turnstile> (Atom p [t \<cdot> \<sigma>. t \<leftarrow> ts])\<close>
+    by auto
+  also have \<open>... \<longleftrightarrow> [\<lbrakk>t\<rbrakk>\<^bsup>\<M>,\<beta>\<^esup>. t \<leftarrow> [t \<cdot> \<sigma>. t \<leftarrow> ts]] \<in> interp_rel \<M> p\<close>
+    by auto
+  also have \<open>... \<longleftrightarrow> [\<lbrakk>t \<cdot> \<sigma>\<rbrakk>\<^bsup>\<M>,\<beta>\<^esup>. t \<leftarrow> ts] \<in> interp_rel \<M> p\<close>
+    using concat_map[of "\<lambda>t. \<lbrakk>t\<rbrakk>\<^bsup>\<M>,\<beta>\<^esup>" "\<lambda>t. t \<cdot> \<sigma>"] by presburger
+  also have \<open>... \<longleftrightarrow> [\<lbrakk>t\<rbrakk>\<^bsup>\<M>,eval_subst \<M> \<beta> \<sigma>\<^esup>. t \<leftarrow> ts] \<in> interp_rel \<M> p\<close>
+    using subst_lemma_terms[of _ \<sigma> \<M> \<beta>] by auto
+  finally show ?case
+    by simp
 next
   case (Forall x \<phi>)
   define \<sigma>' where "\<sigma>' = \<sigma>(x := Var x)"
-  have \<open>FV (\<phi> \<cdot>\<^sub>f\<^sub>m \<sigma>(y := Var z)) - {z} = FV (\<phi> \<cdot>\<^sub>f\<^sub>m \<sigma>) - {y}\<close> for y z
-  proof
-    have \<open>y \<notin> FV (\<phi> \<cdot>\<^sub>f\<^sub>m \<sigma>(y := Var z)) - {z}\<close>
-    proof (rule ccontr)
-      assume \<open>\<not> y \<notin> FV (\<phi> \<cdot>\<^sub>f\<^sub>m \<sigma>(y := Var z)) - {z}\<close>
-      then have \<open>y \<in> FV (\<phi> \<cdot>\<^sub>f\<^sub>m \<sigma>(y := Var z))\<close>
-        by auto
-      then have \<open>Var y \<in> \<sigma>(y := Var z) ` (UNIV::nat set)\<close>
-        sorry
-      then show False
-        sorry
-    qed
-    show \<open>FV (\<phi> \<cdot>\<^sub>f\<^sub>m \<sigma>(y := Var z)) - {z} \<subseteq> FV (\<phi> \<cdot>\<^sub>f\<^sub>m \<sigma>) - {y}\<close>
+  show ?case
+  proof (cases "\<exists> y. y \<in> FV (\<^bold>\<forall> x\<^bold>. \<phi>) \<and> x \<in> FVT (\<sigma>' y)")
+    case False
+    then have \<open>(\<^bold>\<forall> x\<^bold>. \<phi>) \<cdot>\<^sub>f\<^sub>m \<sigma> = \<^bold>\<forall> x\<^bold>. (\<phi> \<cdot>\<^sub>f\<^sub>m \<sigma>')\<close>
+      using formsubst_def_switch \<sigma>'_def by fastforce
+    then have \<open>\<M>,\<beta> \<Turnstile> ((\<^bold>\<forall> x\<^bold>. \<phi>) \<cdot>\<^sub>f\<^sub>m \<sigma>) = (\<forall>a \<in> dom \<M>. \<M>,\<beta>(x := a) \<Turnstile> (\<phi> \<cdot>\<^sub>f\<^sub>m \<sigma>'))\<close>
+      by auto
+    also have \<open>... = (\<forall>a \<in> dom \<M>. \<M>,(\<lambda>v. \<lbrakk>\<sigma>' v\<rbrakk>\<^bsup>\<M>,\<beta>(x := a)\<^esup>) \<Turnstile> \<phi>)\<close>
+      using Forall by blast
+    also have \<open>... = (\<forall>a \<in> dom \<M>. \<M>,(\<lambda>v. \<lbrakk>\<sigma>' v\<rbrakk>\<^bsup>\<M>,\<beta>\<^esup>)(x := a) \<Turnstile> \<phi>)\<close>
     proof
-      fix x
-      assume \<open>x \<in> FV (\<phi> \<cdot>\<^sub>f\<^sub>m \<sigma>(y := Var z)) - {z}\<close>
-      show \<open>x \<in> FV (\<phi> \<cdot>\<^sub>f\<^sub>m \<sigma>) - {y}\<close>
+      assume forward: \<open>\<forall>a \<in> dom \<M>. \<M>,(\<lambda>v. \<lbrakk>\<sigma>' v\<rbrakk>\<^bsup>\<M>,\<beta>(x := a)\<^esup>) \<Turnstile> \<phi>\<close>
+      show \<open>\<forall>a \<in> dom \<M>. \<M>,(\<lambda>v. \<lbrakk>\<sigma>' v\<rbrakk>\<^bsup>\<M>,\<beta>\<^esup>)(x := a) \<Turnstile> \<phi>\<close>
+      proof
+        fix a
+        assume \<open>a \<in> dom \<M>\<close>
+        then have \<open>\<M>,(\<lambda>v. \<lbrakk>\<sigma>' v\<rbrakk>\<^bsup>\<M>,\<beta>(x := a)\<^esup>) \<Turnstile> \<phi>\<close>
+          using forward by blast
+        show \<open>\<M>,(\<lambda>v. \<lbrakk>\<sigma>' v\<rbrakk>\<^bsup>\<M>,\<beta>\<^esup>)(x := a) \<Turnstile> \<phi>\<close>
+          using subst_lemma_terms
+          sorry
+      qed
+    next
+      assume \<open>\<forall>a \<in> dom \<M>. \<M>,(\<lambda>v. \<lbrakk>\<sigma>' v\<rbrakk>\<^bsup>\<M>,\<beta>\<^esup>)(x := a) \<Turnstile> \<phi>\<close>
+      show \<open>\<forall>a \<in> dom \<M>. \<M>,(\<lambda>v. \<lbrakk>\<sigma>' v\<rbrakk>\<^bsup>\<M>,\<beta>(x := a)\<^esup>) \<Turnstile> \<phi>\<close>
         sorry 
     qed
+    then show ?thesis sorry
   next
-    show \<open>FV (\<phi> \<cdot>\<^sub>f\<^sub>m \<sigma>) - {y} \<subseteq> FV (\<phi> \<cdot>\<^sub>f\<^sub>m \<sigma>(y := Var z)) - {z}\<close>
-    proof
-      fix x
-      assume \<open>x \<in> FV (\<phi> \<cdot>\<^sub>f\<^sub>m \<sigma>) - {y}\<close>
-      show \<open>x \<in> FV (\<phi> \<cdot>\<^sub>f\<^sub>m \<sigma>(y := Var z)) - {z}\<close>
-        sorry
-    qed
-  qed
-  show ?case
-  proof (cases \<open>\<exists> y. y \<in> FV (\<^bold>\<forall> x\<^bold>. \<phi>) \<and> x \<in> FVT (\<sigma>' y)\<close>)
     case True
-    then have \<open>FV ((\<^bold>\<forall> x\<^bold>. \<phi>) \<cdot>\<^sub>f\<^sub>m \<sigma>) =
-      FV ((let z = variant (FV (\<^bold>\<forall> x\<^bold>. \<phi>)) in \<^bold>\<forall> z\<^bold>. (\<phi> \<cdot>\<^sub>f\<^sub>m \<sigma>(x := Var z))))\<close>
-      by (simp add: \<sigma>'_def)
-    also have \<open>... = (let z = variant (FV (\<^bold>\<forall> x\<^bold>. \<phi>)) in FV (\<phi> \<cdot>\<^sub>f\<^sub>m \<sigma>(x := Var z)) - {z})\<close>
-      by (meson FV.simps(4))
-    also have \<open>... = FV (\<phi> \<cdot>\<^sub>f\<^sub>m \<sigma>) - {x}\<close>
-      sorry
-    then show ?thesis sorry
-  next
-    case False
     then show ?thesis sorry
   qed
-qed
+
+qed auto
 
 
 end
